

$$Q(z) = P(z)$$

$$Q_N(z) = P_N(z)$$

$$P(N+1) = P(N) + \sum_{k=0}^{N+1} \binom{N+1}{k} z^{N+1-k} \cdot z_0^k a_{N+1}$$

$$A(N) : \underbrace{\sum_{n=0}^N z^n \sum_{k=0}^{N-n} a_{n+k} \binom{n+k}{k} \cdot z_0^k}_{Q(N)} = \underbrace{\sum_{n=0}^N \sum_{k=0}^n \binom{n}{k} z^{n-k} \cdot z_0^k a_n}_{P(N)}$$

$$\begin{aligned} \Rightarrow Q(N+1) &= \sum_{n=0}^{N+1} z^n \sum_{k=0}^{N+1-n} a_{n+k} \binom{n+k}{k} \cdot z_0^k \\ &= \sum_{n=0}^N z^n \left(\sum_{k=0}^{N-n} a_{n+k} \binom{n+k}{k} \cdot z_0^k + \underbrace{a_{N+1} \binom{N+1}{N+1-n} \cdot z_0^{N+1-n}}_{k=N+1-n} \right) + \underbrace{z^{N+1} \cdot a_{N+1} \binom{N+1}{0}}_{n=N+1} \\ &= \underbrace{\sum_{n=0}^N z^n \sum_{k=0}^{N-n} a_{n+k} \binom{n+k}{k} \cdot z_0^k}_{P(N)} + z^N a_{N+1} \binom{N+1}{N+1-N} z_0^{N+1-N} + \underbrace{z^{N+1} a_{N+1} \binom{N+1}{0}}_{n=N+1} \\ &= \underbrace{\sum_{n=0}^N \sum_{k=0}^n \binom{n}{k} z^{n-k} \cdot z_0^k a_n}_{P(N)} + z^N a_{N+1} \binom{N+1}{N+1-N} z_0^{N+1-N} \\ &= P(N) + \sum_{k=0}^N z^k a_{N+1} z_0^{N+1-k} \binom{N+1}{N+1-k} \\ &= P(N) + \sum_{k=0}^{N+1} z^k a_{N+1} z_0^{N+1-k} \binom{N+1}{N+1-k} \\ &= P(N) + \sum_{k=0}^{N+1} z^{N+1-k} a_{N+1} z_0^k \binom{N+1}{k} \\ &= \sum_{n=0}^N \sum_{k=0}^n \binom{n}{k} z^{n-k} \cdot z_0^k \cdot a_n + \sum_{k=0}^{N+1} \binom{N+1}{k} z^{N+1-k} \cdot z_0^k a_{N+1} \\ &= P(N+1) \end{aligned}$$

$$P(N+1) = P(N) + \sum_{k=0}^{N+1} \binom{N+1}{k} z^{N+1-k} \cdot z_0^k a_{N+1}$$